Splay trees can now be used with just A -> A -> bool instead of Ord. Implemented general self-balancing BSTs and proved the necessary lemmas, but not sure yet if all the desired trees (red-black, AVL etc.) are derivable from them.

DS/BST/SplayTree2.v
@@ -1,90 +1,111 @@
-Require Export BTree.
-Require Import BST.
 Require Export Ord.
-Require Export Sorting.Sort.
+Require Import BST.
 
 Set Implicit Arguments.
 
-Definition SplayTree (A : Ord) : Type := BTree A.
+Definition SplayTree (A : Type) : Type := BTree A.
 
 Function smaller
-  {A : Ord} (pivot : A) (h : SplayTree A) : SplayTree A :=
+  {A : Type} (leb : A -> A -> bool) (pivot : A) (h : SplayTree A) : SplayTree A :=
 match h with
     | empty => empty
     | node v l r =>
-        if v ≤? pivot
+        if leb v pivot
         then
           match r with
               | empty => node v l empty
               | node v' l' r' =>
-                  if v' ≤? pivot
+                  if leb v' pivot
                   then (* v <= v' <= pivot *)
-                    node v' (node v l l') (smaller pivot r')
+                    node v' (node v l l') (smaller leb pivot r')
                   else (* v <= pivot < v' *)
-                    node v l (smaller pivot l')
+                    node v l (smaller leb pivot l')
           end
-        else smaller pivot l
+        else smaller leb pivot l
 end.
 
 Function bigger
-  {A : Ord} (pivot : A) (h : SplayTree A) : SplayTree A :=
+  {A : Type} (leb : A -> A -> bool) (pivot : A) (h : SplayTree A) : SplayTree A :=
 match h with
     | empty => empty
     | node v l r =>
-        if v ≤? pivot
-        then bigger pivot r
+        if leb v pivot
+        then bigger leb pivot r
         else
           match l with
               | empty => node v empty r
               | node v' l' r' =>
-                  if v' ≤? pivot
+                  if leb v' pivot
                   then (* v' <= pivot < v *)
-                    node v (bigger pivot r') r
+                    node v (bigger leb pivot r') r
                   else (* pivot < v' <= v *)
-                    node v' (bigger pivot l') (node v r' r)
+                    node v' (bigger leb pivot l') (node v r' r)
           end
 end.
 
 Definition splay
-  {A : Ord} (x : A) (h : SplayTree A) : SplayTree A * SplayTree A:=
-    (smaller x h, bigger x h).
+  {A : Type} (leb : A -> A -> bool) (pivot : A) (h : SplayTree A) : SplayTree A * SplayTree A:=
+    (smaller leb pivot h, bigger leb pivot h).
 
 Definition insert
-  {A : Ord} (x : A) (h : SplayTree A) : SplayTree A :=
-    let (smaller, bigger) := splay x h
+  {A : Type} (leb : A -> A -> bool) (x : A) (h : SplayTree A) : SplayTree A :=
+    let (smaller, bigger) := splay leb x h
     in node x smaller bigger.
 
-Function merge {A : Ord} (h1 h2 : SplayTree A) : SplayTree A :=
+Function merge {A : Type} (leb : A -> A -> bool) (h1 h2 : SplayTree A) : SplayTree A :=
 match h1 with
     | empty => h2
     | node v l r =>
-        let '(l', r') := splay v h2
-        in node v (merge l l') (merge r r')
+        let '(l', r') := splay leb v h2
+        in node v (merge leb l l') (merge leb r r')
 end.
 
+(** We can use [removeMin] and [remove] from BST.v *)
+(* Print removeMin. *)
+(* Print remove. *)
+
 (** Properties [bigger]. *)
+
+Lemma isEmpty_bigger_true :
+  forall {A : Type} (leb : A -> A -> bool) (x : A) (h : SplayTree A),
+    isEmpty h = true -> isEmpty (bigger leb x h) = true.
+Proof.
+  intros.
+  functional induction smaller leb x h;
+  cbn in *; congruence.
+Qed.
+
+Lemma isEmpty_bigger_false :
+  forall {A : Type} (leb : A -> A -> bool) (x : A) (h : SplayTree A),
+    isEmpty (bigger leb x h) = false -> isEmpty h = false.
+Proof.
+  intros.
+  functional induction smaller leb x h;
+  cbn in *; congruence.
+Qed.
 
 Lemma Elem_bigger :
   forall {A : Ord} {pivot : A} {h : SplayTree A},
     isBST cmp h ->
       forall x : A,
-        Elem x (bigger pivot h)
+        Elem x (bigger cmp pivot h)
           <->
         Elem x h /\ x > pivot.
 Proof.
   intros until h.
-  functional induction bigger pivot h;
+  functional induction bigger cmp pivot h;
   isBST; intro;
   rewrite ?Elem_node, ?IHs; auto;
+  unfold comparison2bool in *;
   split; Elems'.
 Qed.
 
 Lemma isBST_bigger :
   forall (A : Ord) (pivot : A) (h : SplayTree A),
-    isBST cmp h -> isBST cmp (bigger pivot h).
+    isBST cmp h -> isBST cmp (bigger cmp pivot h).
 Proof.
   intros until h.
-  functional induction bigger pivot h;
+  functional induction bigger cmp pivot h;
   isBST'; auto; intros.
     apply Elem_bigger in H; firstorder.
     apply Elem_bigger in H; firstorder.
@@ -95,27 +116,46 @@ Qed.
 
 (** Properties of [smaller]. *)
 
+Lemma isEmpty_smaller_true :
+  forall {A : Type} (leb : A -> A -> bool) (x : A) (h : SplayTree A),
+    isEmpty h = true -> isEmpty (smaller leb x h) = true.
+Proof.
+  intros.
+  functional induction smaller leb x h;
+  cbn in *; congruence.
+Qed.
+
+Lemma isEmpty_smaller_false :
+  forall {A : Type} {leb : A -> A -> bool} {x : A} {h : SplayTree A},
+    isEmpty (smaller leb x h) = false -> isEmpty h = false.
+Proof.
+  intros.
+  functional induction smaller leb x h;
+  cbn in *; congruence.
+Qed.
+
 Lemma Elem_smaller : (* TODO: fix definition of isBST *)
   forall {A : Ord} {pivot : A} {h : SplayTree A},
     isBST cmp h ->
       forall x : A,
-        Elem x (smaller pivot h)
+        Elem x (smaller cmp pivot h)
           <->
         Elem x h /\ x < pivot.
 Proof.
   intros until h.
-  functional induction smaller pivot h;
+  functional induction smaller cmp pivot h;
   isBST; intro;
   rewrite ?Elem_node, ?IHs; auto;
+  unfold comparison2bool in *;
   split; Elems'.
 Admitted.
 
 Lemma isBST_smaller :
   forall {A : Ord} {pivot : A} {h : SplayTree A},
-    isBST cmp h -> isBST cmp (smaller pivot h).
+    isBST cmp h -> isBST cmp (smaller cmp pivot h).
 Proof.
   intros until h.
-  functional induction smaller pivot h;
+  functional induction smaller cmp pivot h;
   isBST'; try intro;
   rewrite ?Elem_smaller; Elems'.
     specialize (H6 v' ltac:(auto)). trich.
@@ -124,9 +164,25 @@ Qed.
 
 (** Properties of [splay]. *)
 
+Lemma isEmpty_splay :
+  forall {A : Type} {leb : A -> A -> bool} {x : A} {h l r : SplayTree A},
+    splay leb x h = (l, r) ->
+      isEmpty h = isEmpty l && isEmpty r.
+Proof.
+  intros until h.
+  unfold splay. inv 1.
+  functional induction smaller leb x h;
+  try destruct l; cbn; trich.
+    destruct (leb v x); cbn in *; congruence.
+    destruct l2, (leb v x), (leb a x); cbn; trich.
+      rewrite andb_false_r. reflexivity.
+      destruct (leb a0 x); reflexivity.
+      rewrite andb_false_r. reflexivity.
+Qed.
+
 Lemma Elem_splay :
   forall {A : Ord} {pivot : A} {h l r : SplayTree A},
-    splay pivot h = (l, r) ->
+    splay cmp pivot h = (l, r) ->
       isBST cmp h ->
         forall x : A, Elem x h <-> Elem x l \/ Elem x r.
 Proof.
@@ -142,7 +198,7 @@ Admitted.
 
 Lemma isBST_splay :
   forall {A : Ord} {pivot : A} {h l r : SplayTree A},
-    splay pivot h = (l, r) ->
+    splay cmp pivot h = (l, r) ->
       isBST cmp h -> isBST cmp (node pivot l r).
 Proof.
   unfold splay.
@@ -155,10 +211,19 @@ Qed.
 
 (** Properties of [insert]. *)
 
+Lemma isEmpty_insert :
+  forall {A : Type} (leb : A -> A -> bool) (x : A) (h : SplayTree A),
+    isEmpty (insert leb x h) = false.
+Proof.
+  intros. unfold insert.
+  destruct (splay leb x h).
+  cbn. reflexivity.
+Qed.
+
 Lemma Elem_insert :
   forall {A : Ord} {x : A} {h : SplayTree A},
     isBST cmp h ->
-      forall y : A, Elem y (insert x h) <-> y = x \/ Elem y h.
+      forall y : A, Elem y (insert cmp x h) <-> y = x \/ Elem y h.
 Proof.
   unfold insert, splay. intros.
   rewrite Elem_node, Elem_smaller, Elem_bigger; auto. split.
@@ -168,25 +233,32 @@ Qed.
 
 Lemma isBST_insert :
   forall {A : Ord} {x : A} {h : SplayTree A},
-    isBST cmp h -> isBST cmp (insert x h).
+    isBST cmp h -> isBST cmp (insert cmp x h).
 Proof.
   intros.
   unfold insert.
-  destruct (splay x h) eqn: Heq.
+  destruct (splay cmp x h) eqn: Heq.
   eapply isBST_splay; eassumption.
 Qed.
 
 (** Properties of [merge]. *)
 
+Lemma isEmpty_merge :
+  forall {A : Type} (leb : A -> A -> bool) (h1 h2 : SplayTree A),
+    isEmpty (merge leb h1 h2) = isEmpty h1 && isEmpty h2.
+Proof.
+  destruct h1; cbn; reflexivity.
+Qed.
+
 Lemma Elem_merge :
   forall {A : Ord} {h1 h2 : SplayTree A} {x : A},
     isBST cmp h1 -> isBST cmp h2 ->
-      Elem x (merge h1 h2)
+      Elem x (merge cmp h1 h2)
         <->
       Elem x h1 \/ Elem x h2.
 Proof.
   intros until h2.
-  functional induction merge h1 h2;
+  functional induction merge cmp h1 h2;
   intro; isBST.
     split; Elems.
     {
@@ -199,10 +271,10 @@ Qed.
 Lemma isBST_merge :
   forall {A : Ord} {h1 h2 : SplayTree A},
     isBST cmp h1 -> isBST cmp h2 ->
-      isBST cmp (merge h1 h2).
+      isBST cmp (merge cmp h1 h2).
 Proof.
   intros until h2.
-  functional induction merge h1 h2;
+  functional induction merge cmp h1 h2;
   isBST.
     assumption.
     pose (isBST_splay e0 H). isBST'.
@@ -210,70 +282,4 @@ Proof.
       intro. rewrite Elem_merge; Elems.
       apply IHs0; assumption.
       intro. rewrite Elem_merge; Elems.
-Qed.
-
-(** Properties of [isEmpty] *)
-
-Lemma isEmpty_smaller_true :
-  forall (A : Ord) (x : A) (h : SplayTree A),
-    isEmpty h = true -> isEmpty (smaller x h) = true.
-Proof.
-  intros.
-  functional induction smaller x h;
-  cbn in *; congruence.
-Qed.
-
-Lemma isEmpty_smaller_false :
-  forall (A : Ord) (x : A) (h : SplayTree A),
-    isEmpty (smaller x h) = false -> isEmpty h = false.
-Proof.
-  intros.
-  functional induction smaller x h;
-  cbn in *; congruence.
-Qed.
-
-Lemma isEmpty_bigger_true :
-  forall (A : Ord) (x : A) (h : SplayTree A),
-    isEmpty h = true -> isEmpty (bigger x h) = true.
-Proof.
-  intros.
-  functional induction smaller x h;
-  cbn in *; congruence.
-Qed.
-
-Lemma isEmpty_bigger_false :
-  forall (A : Ord) (x : A) (h : SplayTree A),
-    isEmpty (bigger x h) = false -> isEmpty h = false.
-Proof.
-  intros.
-  functional induction smaller x h;
-  cbn in *; congruence.
-Qed.
-
-Lemma isEmpty_splay :
-  forall {A : Ord} {x : A} {h l r : SplayTree A},
-    splay x h = (l, r) ->
-      isEmpty h = isEmpty l && isEmpty r.
-Proof.
-  intros until h.
-  unfold splay. inv 1.
-  functional induction smaller x h;
-  try destruct l; cbn; trich.
-    destruct l2; cbn; trich.
-    trich. rewrite andb_false_r. reflexivity.
-Qed.
-
-Lemma isEmpty_insert :
-  forall (A : Ord) (x : A) (h : SplayTree A),
-    isEmpty (insert x h) = false.
-Proof.
-  intros. unfold insert. case_eq (splay x h); intros small big H.
-  cbn. reflexivity.
-Qed.
-
-Lemma isEmpty_merge :
-  forall {A : Ord} {h1 h2 : SplayTree A},
-    isEmpty (merge h1 h2) = isEmpty h1 && isEmpty h2.
-Proof.
-  destruct h1; cbn; reflexivity.
 Qed.
