DS/BST/Balanced.v
@@ -1,0 +1,266 @@
+Require Export RCCBase.
+Require Export Ord.
+Require Export EBTree.
+
+Class BalanceArgs (A : Ord) : Type :=
+{
+    B : Type;
+    default : B;
+    balance :
+      forall (b : B) (l : EBTree B A) (v : A) (r : EBTree B A),
+        EBTree B A;
+    isEmpty_balance :
+      forall (b : B) (l : EBTree B A) (v : A) (r : EBTree B A),
+        isEmpty (balance b l v r) = false;
+    Elem_balance :
+      forall (b : B) (x v : A) (l r : EBTree B A),
+        Elem x (balance b l v r) <-> Elem x l \/ x = v \/ Elem x r;
+    isBST_balance :
+      forall (b : B) (v : A) (l r : EBTree B A),
+        isBST (N b l v r) -> isBST (balance b l v r);
+}.
+
+(* Coercion A : BalanceArgs >-> Ord. *)
+(* Coercion A : BalanceArgs >-> Sortclass. *)
+
+Definition BalancedBTree {A : Ord} (args : BalanceArgs A) : Type := EBTree B A.
+
+Definition leaf
+  {A : Ord} {args : BalanceArgs A}
+  (x : A) : BalancedBTree args :=
+    N default E x E.
+
+Function insert
+  {A : Ord} {args : BalanceArgs A}
+  (x : A) (t : BalancedBTree args) : BalancedBTree args :=
+match t with
+    | E => N default E x E
+    | N b l v r =>
+        if x ≤? v
+        then balance b (insert x l) v r
+        else balance b l v (insert x r)
+end.
+
+Function removeMin
+  {A : Ord} {args : BalanceArgs A}
+  (t : BalancedBTree args)
+    : option (A * BalancedBTree args) :=
+match t with
+    | E         => None
+    | N b l v r =>
+        match removeMin l with
+            | None => Some (v, r)
+            | Some (m, l') => Some (m, balance b l' v r)
+        end
+end.
+
+Function remove
+  {A : Ord} {args : BalanceArgs A}
+  (x : A) (t : BalancedBTree args)
+    : BalancedBTree args :=
+match t with
+    | E         => E
+    | N b l v r =>
+        match cmp x v with
+            | Lt => balance b (remove x l) v r
+            | Gt => balance b l v (remove x r)
+            | Eq => 
+                match removeMin r with
+                    | None         => l
+                    | Some (m, r') => balance b l m r'
+                end
+        end
+end.
+
+Fixpoint fromList
+  {A : Ord} {args : BalanceArgs A}
+  (l : list A) : BalancedBTree args :=
+match l with
+    | [] => E
+    | h :: t => insert h (fromList t)
+end.
+
+(** Properties of [leaf]. *)
+
+Lemma Elem_leaf :
+  forall {A : Ord} {args : BalanceArgs A} (x y : A),
+    Elem x (leaf y) <-> x = y.
+Proof.
+  unfold leaf. split.
+    inv 1; inv H1.
+    intros ->. auto.
+Qed.
+
+Lemma isBST_leaf :
+  forall {A : Ord} {args : BalanceArgs A} (x : A),
+    isBST (leaf x).
+Proof.
+  unfold leaf. intros. constructor; auto; inv 1.
+Qed.
+
+Lemma isBST2_leaf :
+  forall {A : Ord} {args : BalanceArgs A} (x : A),
+    isBST2 (leaf x).
+Proof.
+  constructor; auto.
+Qed.
+
+(** Properties of [insert]. *)
+
+Lemma isEmpty_insert :
+  forall
+    {A : Ord} {args : BalanceArgs A}
+    (x : A) (t : BalancedBTree args),
+      isEmpty (insert x t) = false.
+Proof.
+  intros.
+  functional induction insert x t;
+  cbn.
+    reflexivity.
+    apply isEmpty_balance.
+    apply isEmpty_balance.
+Qed.
+
+Lemma Elem_insert :
+  forall
+    {A : Ord} {args : BalanceArgs A}
+    (x y : A) (t : BalancedBTree args),
+      Elem x (insert y t) <-> x = y \/ Elem x t.
+Proof.
+  intros until t. revert x.
+  functional induction insert y t;
+  intros.
+    split; inv 1.
+    rewrite Elem_balance, IHb, Elem_N. split; firstorder.
+    rewrite Elem_balance, IHb, Elem_N. split; firstorder.
+Qed.
+
+Lemma isBST_insert :
+  forall
+    {A : Ord} {args : BalanceArgs A}
+    (x : A) (t : BalancedBTree args),
+      isBST t -> isBST (insert x t).
+Proof.
+  intros until t.
+  functional induction insert x t;
+  inv 1.
+    apply isBST_leaf.
+    apply isBST_balance. constructor; auto.
+      intros. rewrite Elem_insert in H. inv H. trich.
+    apply isBST_balance. constructor; auto.
+      intros. rewrite Elem_insert in H. inv H. trich.
+Qed.
+
+(* Lemma isBST2_insert :
+  forall
+    {A : Ord} {args : BalanceArgs A}
+    (x : A) (t : BalancedBTree args),
+      isBST2 t -> isBST2 (insert x t).
+Proof.
+  intros until t.
+  functional induction insert x t;
+  inv 1.
+    apply isBST2_balance. constructor; auto.
+      intros. rewrite Elem_insert in H. inv H. trich.
+    apply isBST2_balance. constructor; auto.
+      intros. rewrite Elem_insert in H. inv H. trich.
+Qed.
+ *)
+
+(** * Properties of [removeMin]. *)
+
+Lemma Elem_removeMin :
+  forall
+    {A : Ord} {args : BalanceArgs A}
+    {t t' : BalancedBTree args} {m : A},
+      removeMin t = Some (m, t') ->
+        forall x : A, Elem x t <-> x = m \/ Elem x t'.
+Proof.
+  intros until t.
+  functional induction removeMin t;
+  inv 1; intro.
+    functional inversion e0; subst.
+      rewrite Elem_N. split; inv 1. inv H0. inv H.
+    rewrite Elem_N, Elem_balance, (IHo _ _ e0).
+      split; intro H; decompose [or] H; clear H; auto.
+Qed.
+
+Lemma isBST_removeMin :
+  forall
+    {A : Ord} {args : BalanceArgs A}
+    (t t' : BalancedBTree args) (m : A),
+      removeMin t = Some (m, t') ->
+        isBST t -> isBST t'.
+Proof.
+  intros until t.
+  functional induction removeMin t;
+  inv 1; inv 1.
+  {
+    specialize (IHo _ _ e0 H5).
+    apply isBST_balance.
+    constructor; auto.
+    intros. apply H4.
+    rewrite (Elem_removeMin e0).
+    right. assumption.
+  }
+Qed.
+
+Lemma removeMin_spec :
+  forall
+    {A : Ord} {args : BalanceArgs A}
+    {t t' : BalancedBTree args} {m : A},
+      removeMin t = Some (m, t') ->
+        isBST t -> forall x : A, Elem x t -> m ≤ x.
+Proof.
+  intros until t.
+  functional induction removeMin t;
+  inv 1; inv 1; intro x.
+    functional inversion e0; subst. inv 1.
+      trich.
+      inv H1.
+    inv 1.
+      apply H4. rewrite (Elem_removeMin e0). auto.
+      specialize (H4 _ H1). specialize (IHo _ _ e0 H5 _ H1). trich.
+      specialize (H6 _ H1). assert (m0 ≤ v).
+        apply H4. rewrite (Elem_removeMin e0). auto.
+        trich.
+Qed.
+
+(** * Properties of [remove] *)
+
+Lemma Elem_remove :
+  forall
+    {A : Ord} {args : BalanceArgs A}
+    {t : BalancedBTree args} {x : A},
+      isBST t ->
+        forall y : A, Elem y (remove x t) -> Elem y t.
+Proof.
+  intros until x.
+  functional induction remove x t;
+  inv 1; intros y;
+  rewrite Elem_balance, Elem_N.
+    specialize (IHb H5 y). firstorder.
+    specialize (IHb H7 y). firstorder.
+    pose (Elem_removeMin e1 y). firstorder.
+Qed.
+
+Lemma isBST_remove :
+  forall
+    {A : Ord} {args : BalanceArgs A}
+    (t : BalancedBTree args) (x : A),
+      isBST t -> isBST (remove x t).
+Proof.
+  intros until x.
+  functional induction remove x t;
+  inv 1.
+    apply isBST_balance. constructor; auto.
+      intros. apply H4. eapply Elem_remove; eassumption.
+    apply isBST_balance. constructor; auto.
+      intros. apply H6. eapply Elem_remove; eassumption.
+    apply isBST_balance. constructor; trich; intros.
+      specialize (H4 _ H). assert (v ≤ m).
+        apply H6. rewrite (Elem_removeMin e1). auto.
+        trich.
+      apply (removeMin_spec e1); auto. rewrite (Elem_removeMin e1). auto.
+      eapply isBST_removeMin; eassumption.
+Qed.
